pulse/src/checker/Pulse.Checker.While.fst
@@ -159,28 +159,28 @@ let tm_l_true : term = FStar.Reflection.V2.Formula.(formula_as_term True_)
 let tm_l_or (a b: term) : term = FStar.Reflection.V2.Formula.(formula_as_term (Or a b))
 let tm_l_and (a b: term) : term = FStar.Reflection.V2.Formula.(formula_as_term (And a b))
 
-let cont_req_marker_lid = Pulse.Reflection.Util.mk_pulse_lib_core_lid "continue_requires_marker"
-let mk_cont_req_marker p = R.pack_ln (R.Tv_App (R.pack_ln (R.Tv_FVar (R.pack_fv cont_req_marker_lid))) (p, R.Q_Explicit))
+let loop_requires_marker_lid = Pulse.Reflection.Util.mk_pulse_lib_core_lid "continue_requires_marker"
+let mk_loop_requires_marker p = R.pack_ln (R.Tv_App (R.pack_ln (R.Tv_FVar (R.pack_fv loop_requires_marker_lid))) (p, R.Q_Explicit))
 
-let rec subst_cont_req_marker (t: term) (v: term -> term) : Dv term =
+let rec subst_loop_requires_marker (t: term) (v: term -> term) : Dv term =
   match R.inspect_ln t with
   | R.Tv_App hd arg -> (
     let default () : Dv term =
-      R.pack_ln (R.Tv_App (subst_cont_req_marker hd v) (subst_cont_req_marker (fst arg) v, snd arg)) in
+      R.pack_ln (R.Tv_App (subst_loop_requires_marker hd v) (subst_loop_requires_marker (fst arg) v, snd arg)) in
     match R.inspect_ln hd with
     | R.Tv_FVar fv ->
-      if R.inspect_fv fv = cont_req_marker_lid then
+      if R.inspect_fv fv = loop_requires_marker_lid then
         v (fst arg)
       else
         default ()
     | _ -> default ()
   )
   | R.Tv_Abs b body ->
-    R.pack_ln (R.Tv_Abs b (subst_cont_req_marker body v))
+    R.pack_ln (R.Tv_Abs b (subst_loop_requires_marker body v))
   | _ -> t
 
-let subst_cont_req_marker_with_true t = subst_cont_req_marker t fun _ -> tm_l_true
-let reduce_cont_req_marker t = subst_cont_req_marker t id
+let subst_loop_requires_marker_with_true t = subst_loop_requires_marker t fun _ -> tm_l_true
+let reduce_loop_requires_marker t = subst_loop_requires_marker t id
 
 #push-options "--fuel 0 --ifuel 0 --z3rlimit_factor 16"
 module RT = FStar.Reflection.Typing
@@ -197,10 +197,10 @@ let check_nuwhile
   : T.Tac (checker_result_t g pre post_hint) =
 
   let g = push_context "nu while loop" t.range g in
-  let Tm_NuWhile { invariant=inv; cont_req; condition=cond; body } = t.term in
+  let Tm_NuWhile { invariant=inv; loop_requires; condition=cond; body } = t.term in
   let inv =
-    if cont_req `eq_tm` tm_l_true then inv else
-    (inv `tm_star` tm_pure (mk_cont_req_marker cont_req)) in
+    if loop_requires `eq_tm` tm_l_true then inv else
+    (inv `tm_star` tm_pure (mk_loop_requires_marker loop_requires)) in
   let (| inv, inv_typing |) =
     purify_and_check_spec (push_context "invariant" (term_range inv) g)
       { ctxt_now = pre; ctxt_old = Some pre }
@@ -227,7 +227,7 @@ let check_nuwhile
       let (| x_cond, g1', (| _, _, t_typ |), (| cond_post, _ |), k |) = res_cond in
       let break_inv = 
         (mk_eq2 u0 tm_bool (term_of_nvar (ppname_default, x_cond)) tm_false
-            `tm_l_and` cont_req)
+            `tm_l_and` loop_requires)
           `tm_l_or` break_inv in
       let break_inv = purify_term g1' { ctxt_now = cond_post; ctxt_old = Some pre } break_inv in
       let break_inv = RU.beta_lax (elab_env g1') break_inv in
@@ -241,7 +241,7 @@ let check_nuwhile
       let break_inv_typ: tot_typing g1'' break_inv tm_slprop = RU.magic () in
       let unit_typ: universe_of g1'' tm_unit u0 = RU.magic () in
       let break_inv = Pulse.JoinComp.infer_post' g1 g1'' y unit_typ break_inv_typ in
-      let break_inv = subst_cont_req_marker_with_true break_inv.post in
+      let break_inv = subst_loop_requires_marker_with_true break_inv.post in
       let break_inv = open_term' break_inv unit_const 0 in
       let break_inv_typ: tot_typing g1 break_inv tm_slprop = RU.magic () in
       (| break_inv, break_inv_typ |)
@@ -281,7 +281,7 @@ let check_nuwhile
   assert (comp_body == comp_nuwhile_body inv body_pre_open);
   let inv_typing2 : tot_typing g2 inv tm_slprop = RU.magic () in
 
-  let while = wtag (Some STT) (Tm_NuWhile { invariant = inv; cont_req = tm_unknown; condition = cond; body }) in
+  let while = wtag (Some STT) (Tm_NuWhile { invariant = inv; loop_requires = tm_unknown; condition = cond; body }) in
   let d: st_typing g2 while (comp_nuwhile inv body_pre_open) =
     T_NuWhile g2 inv body_pre_open cond body inv_typing2 (body_typing_ex body_open_pre_typing) cond_typing body_typing in
   let C_ST cst = comp_nuwhile inv body_pre_open in
