pulse/test/Break.fst
@@ -8,7 +8,7 @@ fn simple_break ()
   let mut k = true;
   while (!k)
     invariant live k
-    break requires true
+    ensures true
   {
     break;
   }
@@ -19,7 +19,7 @@ fn break_continue_and_return (which: UInt8.t)
   let mut i = 0ul;
   while (!i `UInt32.lt` 1000ul)
     invariant live i
-    break requires true
+    ensures true
   {
     if (which = 0uy) {
       break;
@@ -47,7 +47,7 @@ fn find_zero_with_break (a: array Int32.t) (sz: SizeT.t)
     invariant live i
     invariant pure (SizeT.v !i <= SizeT.v sz /\
       (forall (j: nat). j < SizeT.v (!i) ==> Seq.index 'va j <> 0l))
-    break requires (SizeT.v !i < SizeT.v sz /\ a.(!i) = 0l)
+    ensures (SizeT.v !i < SizeT.v sz /\ a.(!i) = 0l)
   {
     if (a.(!i) = 0l) {
       break;
